Semantics_Ternary.thy
@@ -385,6 +385,8 @@ subsection{*Equality with @{term "\<gamma>,p\<turnstile> \<langle>rs, s\<rangle>
   lemma simple_imp_good_ruleset: "simple_ruleset rs \<Longrightarrow> good_ruleset rs"
     by(simp add: simple_ruleset_def good_ruleset_def, fastforce)
 
+  lemma simple_ruleset_tail: "simple_ruleset (r#rs) \<Longrightarrow> simple_ruleset rs" by (simp add: simple_ruleset_def)
+
   lemma simple_ruleset_append: "simple_ruleset (rs\<^sub>1 @ rs\<^sub>2) \<longleftrightarrow> simple_ruleset rs\<^sub>1 \<and> simple_ruleset rs\<^sub>2"
     by(simp add: simple_ruleset_def, blast)
 
